\question % Sample Questions 1, Q9.

\begin{parts}

\part[3]
On the axes in Figure~\ref{fig:graph-of-rational-function}, sketch the graph of $\displaystyle{f(x) = \frac{2}{(x - 1)(x + 1)}}$.

\begin{figure}[h]
    \centering
    \begin{tikzpicture}
    \begin{axis}[
        my axis style,
        height=3.25in,
        xmin=-4.5, xmax=4.5,
        ymin=-9, ymax=9,
        grid=both,
    ]
    \coordinate (A) at (0,-2);
    \ifprintanswers
    \addplot[
        domain=-4:-1.125,
        red,
        <->,
    ] {2/(x^2-1)};
    \addplot[
        domain=-.875:.875,
        red,
        <->,
    ] {2/(x^2-1)};
    \addplot[
        domain=1.125:4,
        red,
        <->,
    ] {2/(x^2-1)} node[near start, right] {$y = f(x)$};
    \fill[red] (A) circle (2pt) node[above] {$(0, -2)$};
    \draw[semithick, dashed, red, <->] (-1,-8.5) -- node[near start, left] {$x = -1$} (-1,8.5);
    \draw[semithick, dashed, red, <->] (1,-8.5) -- node[near start, right] {$x = 1$} (1,8.5);
    \draw[semithick, dashed, red, <->] (-4.25,0) -- node[pos=.15, below] {$y = 0$} (4.25,0);
    \draw[red] (3,-5) node[anchor=west, text width=2in, rounded corners=5pt, fill=white, draw=red] {always include dashed, labelled asymptotes, interesting points, $y = \textrm{such-and-such}$, arrowheads or closed endpoints};
    \else
    \fi
    \end{axis}
    \end{tikzpicture}
    \caption{Sketch the graph here.}
    \label{fig:graph-of-rational-function}
\end{figure}

\part[1]
Show that $\displaystyle{\frac{2}{(x - 1)(x + 1)} = \frac{1}{x - 1} - \frac{1}{x + 1}}$.

\begin{EnvFullwidth}
\begin{solutionorgrid}[1.5in]
The RHS is
\begin{align*}
    \frac{1}{x - 1} - \frac{1}{x + 1} &= \frac{(x + 1) - (x - 1)}{(x - 1)(x + 1)} \\
    &= \frac{2}{(x - 1)(x + 1)},
\end{align*}
which is the LHS.
\end{solutionorgrid}
\end{EnvFullwidth}

\part[1]
Hence, show that $\displaystyle{(f(x))^2 = \frac{1}{(x - 1)^2} + \frac{1}{(x + 1)^2} - \frac{1}{x - 1} + \frac{1}{x + 1}}$.

\begin{EnvFullwidth}
\begin{solutionorgrid}[2in]
We have
\begin{align*}
    (f(x))^2 &= \left(\frac{1}{x - 1} - \frac{1}{x + 1}\right)^{\! 2} \\
    &= \pfrac{1}{x - 1}^{\! 2} - 2 \pfrac{1}{x - 1}\!\pfrac{1}{x + 1} + \pfrac{1}{x + 1}^{\! 2} \\
    &= \frac{1}{(x - 1)^2} - \left(\frac{1}{x - 1} - \frac{1}{x + 1}\right) + \frac{1}{(x + 1)^2} && (\textrm{by (a)}) \\
    &= \frac{1}{(x - 1)^2} + \frac{1}{(x + 1)^2} - \frac{1}{x - 1} + \frac{1}{x + 1}.
\end{align*}
\end{solutionorgrid}
\end{EnvFullwidth}

\part[4]
Find the \emph{exact} volume of the solid obtained when the region bounded by the graph of $f(x)$ and the $x$-axis on the interval $[2, 3]$ is rotated about the $x$-axis.

\begin{EnvFullwidth}
\begin{solutionorgrid}[4in]
The volume is
\begin{align*}
    V &= \pi \int_2^3 y^2 \dif x \\
    &= \pi \int_2^3 \frac{1}{(x - 1)^2} + \frac{1}{(x + 1)^2} - \frac{1}{x - 1} + \frac{1}{x + 1} \dif x && (\textrm{by (b)}) \\
    &= \pi \Eval{-\frac{1}{x - 1} - \frac{1}{x + 1} - \ln(\abs{x - 1}) + \ln(\abs{x + 1})}{2}{3} \\
    &= \pi \Eval{\ln\!\pfrac{x + 1}{x - 1} - \frac{2x}{x^2 - 1}}{2}{3} && (x > 0) \\
    &= \pi \left(\ln\!\pfrac{4}{2} - \frac{6}{8} - \left(\ln\!\pfrac{3}{1} - \frac{4}{3}\right)\right) \\
    &= \pi\left(\ln\!\pfrac{2}{3} + \frac{7}{12}\right) \, \textrm{units}^3.
\end{align*}
\end{solutionorgrid}
\end{EnvFullwidth}

\end{parts}
